renaming
git-svn-id: https://www.lri.fr/svn/demons/why2/trunk@1040 ecafba89-7d34-45a1-8a0b-92829e960b72

bench/c/good/clash.c
@@ -7,3 +7,69 @@ int g() {
   int y; y = 0 ;
   return y;
 }
+
+
+/*@ ensures (x==0 => \result == 1) && (x !=0 => \result == 2) */
+int f(int x) {
+  if (x == 0) {
+    int y; 
+    y = 1;
+    return y;
+  }
+  else {
+    int y;
+    y = 2;
+    return y;
+  }
+}
+
+
+/*@ ensures (x == 0 => \result == 1) && (x != 0 => \result == 2) */
+int h(int x) {
+  int y;
+  y = 2;
+  if (x == 0) {
+    int y; 
+    y = 1;
+    return y;
+  }
+  return y;
+}
+
+
+typedef struct {
+    int toto;
+    int titi;    
+} S1;
+
+/*@ requires \valid(ma_structure)
+  @ assigns  ma_structure.toto */
+void f1(S1 ma_structure)
+{
+    int toto;
+    toto = 0;
+    ma_structure.toto = toto;
+ }
+
+typedef struct {
+    int fst;
+    int sec;
+} S2;
+
+typedef struct {
+    S2 substruct;
+    int titi;
+} S3;
+
+/*@ requires \valid(ma_structure) && \valid(ma_structure.substruct)
+  @ assigns ma_structure.substruct.fst */
+void f2(S3 ma_structure)
+{
+    S2 substruct;
+    substruct.fst = 0;
+    ma_structure.substruct.fst = substruct.fst;
+ }
+
+
+
+
