bench/c/good/coq/clash_why.v
@@ -3,7 +3,143 @@
 
 Require Export caduceus_spec_why.
 
-(* Why obligation from file "why/clash.why", characters 96-119 *)
+(* Why obligation from file "why/clash.why", characters 145-203 *)
+Lemma f1_impl_po_1 : 
+  forall (ma_structure: pointer),
+  forall (alloc: alloc_table),
+  forall (toto: ((memory) Z)),
+  forall (Pre4: (valid alloc ma_structure)),
+  forall (toto_0_1: Z),
+  forall (Post1: toto_0_1 = 0),
+  forall (Pre3: (valid alloc ma_structure)),
+  forall (toto0: ((memory) Z)),
+  forall (Post7: toto0 = (upd toto ma_structure toto_0_1)),
+  (assigns alloc toto toto0 (pointer_loc ma_structure)).
+Proof.
+intuition.
+Save.
+
+(* Why obligation from file "why/clash.why", characters 645-672 *)
+Lemma f2_impl_po_1 : 
+  forall (ma_structure: pointer),
+  forall (alloc: alloc_table),
+  forall (substruct: ((memory) pointer)),
+  forall (Pre8: (valid alloc ma_structure) /\
+                (valid alloc (acc substruct ma_structure))),
+  forall (alloc0: alloc_table),
+  forall (substruct_0: pointer),
+  forall (Post8: ((valid alloc0 substruct_0) /\ (fresh alloc substruct_0)) /\
+                 (alloc_extends alloc alloc0)),
+  (valid alloc0 substruct_0).
+Proof.
+intuition.
+Save.
+
+(* Why obligation from file "why/clash.why", characters 696-726 *)
+Lemma f2_impl_po_2 : 
+  forall (ma_structure: pointer),
+  forall (alloc: alloc_table),
+  forall (fst: ((memory) Z)),
+  forall (substruct: ((memory) pointer)),
+  forall (Pre8: (valid alloc ma_structure) /\
+                (valid alloc (acc substruct ma_structure))),
+  forall (alloc0: alloc_table),
+  forall (substruct_0: pointer),
+  forall (Post8: ((valid alloc0 substruct_0) /\ (fresh alloc substruct_0)) /\
+                 (alloc_extends alloc alloc0)),
+  forall (Pre7: (valid alloc0 substruct_0)),
+  forall (fst0: ((memory) Z)),
+  forall (Post11: fst0 = (upd fst substruct_0 0)),
+  (valid alloc0 ma_structure).
+Proof.
+intuition.
+apply alloc_extends_valid with alloc; auto.
+Save.
+
+(* Why obligation from file "why/clash.why", characters 735-784 *)
+Lemma f2_impl_po_3 : 
+  forall (ma_structure: pointer),
+  forall (alloc: alloc_table),
+  forall (fst: ((memory) Z)),
+  forall (substruct: ((memory) pointer)),
+  forall (Pre8: (valid alloc ma_structure) /\
+                (valid alloc (acc substruct ma_structure))),
+  forall (alloc0: alloc_table),
+  forall (substruct_0: pointer),
+  forall (Post8: ((valid alloc0 substruct_0) /\ (fresh alloc substruct_0)) /\
+                 (alloc_extends alloc alloc0)),
+  forall (Pre7: (valid alloc0 substruct_0)),
+  forall (fst0: ((memory) Z)),
+  forall (Post11: fst0 = (upd fst substruct_0 0)),
+  forall (Pre6: (valid alloc0 ma_structure)),
+  forall (caduceus_1: pointer),
+  forall (Post6: caduceus_1 = (acc substruct ma_structure)),
+  forall (Pre5: (valid alloc0 substruct_0)),
+  forall (aux_1: Z),
+  forall (Post5: aux_1 = (acc fst0 substruct_0)),
+  (valid alloc0 caduceus_1).
+Proof.
+intuition.
+subst; apply alloc_extends_valid with alloc; auto.
+Save.
+
+(* Why obligation from file "why/clash.why", characters 735-784 *)
+Lemma f2_impl_po_4 : 
+  forall (ma_structure: pointer),
+  forall (alloc: alloc_table),
+  forall (fst: ((memory) Z)),
+  forall (substruct: ((memory) pointer)),
+  forall (Pre8: (valid alloc ma_structure) /\
+                (valid alloc (acc substruct ma_structure))),
+  forall (alloc0: alloc_table),
+  forall (substruct_0: pointer),
+  forall (Post8: ((valid alloc0 substruct_0) /\ (fresh alloc substruct_0)) /\
+                 (alloc_extends alloc alloc0)),
+  forall (Pre7: (valid alloc0 substruct_0)),
+  forall (fst0: ((memory) Z)),
+  forall (Post11: fst0 = (upd fst substruct_0 0)),
+  forall (Pre6: (valid alloc0 ma_structure)),
+  forall (caduceus_1: pointer),
+  forall (Post6: caduceus_1 = (acc substruct ma_structure)),
+  forall (Pre5: (valid alloc0 substruct_0)),
+  forall (aux_1: Z),
+  forall (Post5: aux_1 = (acc fst0 substruct_0)),
+  forall (Pre3: (valid alloc0 caduceus_1)),
+  forall (fst1: ((memory) Z)),
+  forall (Post15: fst1 = (upd fst0 caduceus_1 aux_1)),
+  (assigns alloc fst fst1 (pointer_loc (acc substruct ma_structure))).
+Proof.
+intuition.
+subst.
+Admitted.
+
+(* Why obligation from file "why/clash.why", characters 997-1020 *)
+Lemma f_impl_po_1 : 
+  forall (x: Z),
+  forall (Test2: x = 0),
+  forall (y_0_1: Z),
+  forall (Post4: y_0_1 = 1),
+  forall (result1: Z),
+  forall (Post5: result1 = y_0_1),
+  ((x = 0 -> result1 = 1)) /\ ((x <> 0 -> result1 = 2)).
+Proof.
+intuition.
+Save.
+
+(* Why obligation from file "why/clash.why", characters 1064-1087 *)
+Lemma f_impl_po_2 : 
+  forall (x: Z),
+  forall (Test1: x <> 0),
+  forall (y_1_1: Z),
+  forall (Post1: y_1_1 = 2),
+  forall (result1: Z),
+  forall (Post2: result1 = y_1_1),
+  ((x = 0 -> result1 = 1)) /\ ((x <> 0 -> result1 = 2)).
+Proof.
+intuition.
+Save.
+
+(* Why obligation from file "why/clash.why", characters 1283-1306 *)
 Lemma g_impl_po_1 : 
   forall (y: Z),
   forall (y_0_1: Z),
@@ -11,6 +147,34 @@ Lemma g_impl_po_1 :
   forall (result0: Z),
   forall (Post2: result0 = y_0_1),
   result0 = 0 /\ y = y.
+Proof.
+intuition.
+Save.
+
+(* Why obligation from file "why/clash.why", characters 1542-1565 *)
+Lemma h_impl_po_1 : 
+  forall (x: Z),
+  forall (y_0_1: Z),
+  forall (Post1: y_0_1 = 2),
+  forall (Test2: x = 0),
+  forall (y_1_1: Z),
+  forall (Post3: y_1_1 = 1),
+  forall (result2: Z),
+  forall (Post4: result2 = y_1_1),
+  ((x = 0 -> result2 = 1)) /\ ((x <> 0 -> result2 = 2)).
+Proof.
+intuition.
+Save.
+
+(* Why obligation from file "why/clash.why", characters 1578-1579 *)
+Lemma h_impl_po_2 : 
+  forall (x: Z),
+  forall (y_0_1: Z),
+  forall (Post1: y_0_1 = 2),
+  forall (Test1: x <> 0),
+  forall (result1: Z),
+  forall (Post2: result1 = y_0_1),
+  ((x = 0 -> result1 = 1)) /\ ((x <> 0 -> result1 = 2)).
 Proof.
 intuition.
 Save.
