examples-c/tutorial/coq/search_why.v
@@ -3,7 +3,7 @@
 
 Require Export caduceus_spec_why.
 
-(* Why obligation from file "why/search.why", characters 413-493 *)
+(* Why obligation from file "why/search.why", characters 437-520 *)
 Lemma index_impl_po_1 : 
   forall (t: pointer),
   forall (n: Z),
@@ -11,21 +11,21 @@ Lemma index_impl_po_1 :
   forall (alloc: alloc_table),
   forall (intP: ((memory) Z)),
   forall (Pre6: (valid_range alloc t 0 (n - 1))),
-  forall (i: Z),
-  forall (Post6: i = 0),
+  forall (i_0: Z),
+  forall (Post6: i_0 = 0),
   forall (Variant1: Z),
-  forall (i1: Z),
-  forall (Pre5: Variant1 = (n - i1)),
-  forall (Pre4: 0 <= i1 /\
+  forall (i_0_1: Z),
+  forall (Pre5: Variant1 = (n - i_0_1)),
+  forall (Pre4: 0 <= i_0_1 /\
                 (forall (k:Z),
-                 (0 <= k /\ k < i1 -> (acc intP (shift t k)) <> v))),
-  forall (Test4: i1 < n),
-  (valid alloc (shift t i1)).
+                 (0 <= k /\ k < i_0_1 -> (acc intP (shift t k)) <> v))),
+  forall (Test4: i_0_1 < n),
+  (valid alloc (shift t i_0_1)).
 Proof.
 intuition; subst; auto.
 Save.
 
-(* Why obligation from file "why/search.why", characters 505-511 *)
+(* Why obligation from file "why/search.why", characters 533-539 *)
 Lemma index_impl_po_2 : 
   forall (t: pointer),
   forall (n: Z),
@@ -33,21 +33,21 @@ Lemma index_impl_po_2 :
   forall (alloc: alloc_table),
   forall (intP: ((memory) Z)),
   forall (Pre6: (valid_range alloc t 0 (n - 1))),
-  forall (i: Z),
-  forall (Post6: i = 0),
+  forall (i_0: Z),
+  forall (Post6: i_0 = 0),
   forall (Variant1: Z),
-  forall (i1: Z),
-  forall (Pre5: Variant1 = (n - i1)),
-  forall (Pre4: 0 <= i1 /\
+  forall (i_0_1: Z),
+  forall (Pre5: Variant1 = (n - i_0_1)),
+  forall (Pre4: 0 <= i_0_1 /\
                 (forall (k:Z),
-                 (0 <= k /\ k < i1 -> (acc intP (shift t k)) <> v))),
-  forall (Test4: i1 < n),
-  forall (Pre3: (valid alloc (shift t i1))),
-  forall (Test3: (acc intP (shift t i1)) = v),
+                 (0 <= k /\ k < i_0_1 -> (acc intP (shift t k)) <> v))),
+  forall (Test4: i_0_1 < n),
+  forall (Pre3: (valid alloc (shift t i_0_1))),
+  forall (Test3: (acc intP (shift t i_0_1)) = v),
   (forall (result:unit),
    (result = tt ->
     (forall (result:Z),
-     (result = i1 ->
+     (result = i_0_1 ->
       ((0 <= result /\ result < n -> (acc intP (shift t result)) = v)) /\
       ((result = n ->
         (forall (i:Z), (0 <= i /\ i < n -> (acc intP (shift t i)) <> v)))))))).
@@ -56,7 +56,7 @@ intuition.
 subst ; auto.
 Save.
 
-(* Why obligation from file "why/search.why", characters 527-547 *)
+(* Why obligation from file "why/search.why", characters 556-580 *)
 Lemma index_impl_po_3 : 
   forall (t: pointer),
   forall (n: Z),
@@ -64,22 +64,22 @@ Lemma index_impl_po_3 :
   forall (alloc: alloc_table),
   forall (intP: ((memory) Z)),
   forall (Pre6: (valid_range alloc t 0 (n - 1))),
-  forall (i: Z),
-  forall (Post6: i = 0),
+  forall (i_0: Z),
+  forall (Post6: i_0 = 0),
   forall (Variant1: Z),
-  forall (i1: Z),
-  forall (Pre5: Variant1 = (n - i1)),
-  forall (Pre4: 0 <= i1 /\
+  forall (i_0_1: Z),
+  forall (Pre5: Variant1 = (n - i_0_1)),
+  forall (Pre4: 0 <= i_0_1 /\
                 (forall (k:Z),
-                 (0 <= k /\ k < i1 -> (acc intP (shift t k)) <> v))),
-  forall (Test4: i1 < n),
-  forall (Pre3: (valid alloc (shift t i1))),
-  forall (Test2: (acc intP (shift t i1)) <> v),
-  forall (i2: Z),
-  forall (Post3: i2 = (i1 + 1)),
-  (0 <= i2 /\
-  (forall (k:Z), (0 <= k /\ k < i2 -> (acc intP (shift t k)) <> v))) /\
-  (Zwf 0 (n - i2) (n - i1)).
+                 (0 <= k /\ k < i_0_1 -> (acc intP (shift t k)) <> v))),
+  forall (Test4: i_0_1 < n),
+  forall (Pre3: (valid alloc (shift t i_0_1))),
+  forall (Test2: (acc intP (shift t i_0_1)) <> v),
+  forall (i_0_2: Z),
+  forall (Post3: i_0_2 = (i_0_1 + 1)),
+  (0 <= i_0_2 /\
+  (forall (k:Z), (0 <= k /\ k < i_0_2 -> (acc intP (shift t k)) <> v))) /\
+  (Zwf 0 (n - i_0_2) (n - i_0_1)).
 Proof.
 intuition.
 assert (k<i1 \/ k=i1).
@@ -90,7 +90,7 @@ apply Test2.
 subst; auto.
 Save.
 
-(* Why obligation from file "why/search.why", characters 184-553 *)
+(* Why obligation from file "why/search.why", characters 193-587 *)
 Lemma index_impl_po_4 : 
   forall (t: pointer),
   forall (n: Z),
@@ -98,17 +98,17 @@ Lemma index_impl_po_4 :
   forall (alloc: alloc_table),
   forall (intP: ((memory) Z)),
   forall (Pre6: (valid_range alloc t 0 (n - 1))),
-  forall (i: Z),
-  forall (Post6: i = 0),
+  forall (i_0: Z),
+  forall (Post6: i_0 = 0),
   forall (Variant1: Z),
-  forall (i1: Z),
-  forall (Pre5: Variant1 = (n - i1)),
-  forall (Pre4: 0 <= i1 /\
+  forall (i_0_1: Z),
+  forall (Pre5: Variant1 = (n - i_0_1)),
+  forall (Pre4: 0 <= i_0_1 /\
                 (forall (k:Z),
-                 (0 <= k /\ k < i1 -> (acc intP (shift t k)) <> v))),
-  forall (Test1: i1 >= n),
+                 (0 <= k /\ k < i_0_1 -> (acc intP (shift t k)) <> v))),
+  forall (Test1: i_0_1 >= n),
   (forall (result:Z),
-   (result = i1 ->
+   (result = i_0_1 ->
     ((0 <= result /\ result < n -> (acc intP (shift t result)) = v)) /\
     ((result = n ->
       (forall (i:Z), (0 <= i /\ i < n -> (acc intP (shift t i)) <> v)))))).
@@ -119,7 +119,7 @@ omega.
 subst;auto.
 Save.
 
-(* Why obligation from file "why/search.why", characters 233-373 *)
+(* Why obligation from file "why/search.why", characters 246-393 *)
 Lemma index_impl_po_5 : 
   forall (t: pointer),
   forall (n: Z),
@@ -127,9 +127,10 @@ Lemma index_impl_po_5 :
   forall (alloc: alloc_table),
   forall (intP: ((memory) Z)),
   forall (Pre6: (valid_range alloc t 0 (n - 1))),
-  forall (i: Z),
-  forall (Post6: i = 0),
-  0 <= i /\ (forall (k:Z), (0 <= k /\ k < i -> (acc intP (shift t k)) <> v)).
+  forall (i_0: Z),
+  forall (Post6: i_0 = 0),
+  0 <= i_0 /\
+  (forall (k:Z), (0 <= k /\ k < i_0 -> (acc intP (shift t k)) <> v)).
 Proof.
 intuition.
 Save.
